Issue 230: Added the name field to the Ifcs and derived all other name from it.

Fifo/Ifc.v
@@ -1,16 +1,25 @@
 Require Import Kami.AllNotations.
 Section FifoInterface.
-  Context (k: Kind). 
-  Class Fifo: Type :=
+  Class FifoParams :=
     {
-      getLen: nat;
-      regs: list RegInitT;
-      regFiles: list RegFileBase;
-      isEmpty: forall {ty}, ActionT ty Bool;
-      isFull: forall {ty}, ActionT ty Bool;
-      first: forall {ty}, ActionT ty (Maybe k);
-      deq: forall {ty}, ActionT ty (Maybe k);
-      enq: forall {ty}, ty k -> ActionT ty Bool;
-      flush: forall {ty}, ActionT ty Void
+      name: string;
+      k : Kind;
     }.
+
+  Section fifoParams.
+    Context (fifoParams: FifoParams). 
+
+    Class Fifo: Type :=
+      {
+        getLen: nat;
+        regs: list RegInitT;
+        regFiles: list RegFileBase;
+        isEmpty: forall {ty}, ActionT ty Bool;
+        isFull: forall {ty}, ActionT ty Bool;
+        first: forall {ty}, ActionT ty (Maybe k);
+        deq: forall {ty}, ActionT ty (Maybe k);
+        enq: forall {ty}, ty k -> ActionT ty Bool;
+        flush: forall {ty}, ActionT ty Void
+      }.
+  End fifoParams.
 End FifoInterface.
