FreeList/Ifc.v
@@ -1,17 +1,27 @@
 Require Import Kami.AllNotations.
 Require Import StdLibKami.Fifo.Ifc.
 Section Freelist.
-  Context {len: nat}.
+  Class FreeListParams
+    := {
+         name  : string;
+         tagSz : nat;
+         (* len   := Nat.pow 2 tagSz; *)
+         
+       }.
 
-  Let k := Bit (Nat.log2_up len).
-  Class FreeList: Type :=
-    {
-      regs: list RegInitT;
-      regFiles: list RegFileBase;
-      length: nat;
-      initialize: forall {ty}, ActionT ty Void;
-      nextToAlloc: forall {ty}, ActionT ty (Maybe k);
-      alloc: forall {ty}, ty k -> ActionT ty Bool;
-      free: forall {ty}, ty k -> ActionT ty Void;
-    }.
+  Section freelistParams.
+    Context {freeListParams : FreeListParams}.
+
+    Let k := Bit tagSz. (* (Nat.log2_up len). *)
+    Class FreeList: Type :=
+      {
+        regs: list RegInitT;
+        regFiles: list RegFileBase;
+        length: nat;
+        initialize: forall {ty}, ActionT ty Void;
+        nextToAlloc: forall {ty}, ActionT ty (Maybe k);
+        alloc: forall {ty}, ty k -> ActionT ty Bool;
+        free: forall {ty}, ty k -> ActionT ty Void;
+      }.
+  End freelistParams.
 End Freelist.
