Cam/SimpleCam.v
@@ -3,29 +3,36 @@ Require Import StdLibKami.Cam.Ifc.
 Require Import StdLibKami.ReplacementPolicy.Ifc.
 
 Section cam.
-  Axiom cheat : forall A, A.
+  Context {camParams : CamParams}.
+
+  Local Definition regName := (StdLibKami.Cam.Ifc.name ++ ".regName")%string.
 
   Open Scope kami_expr.
   Open Scope kami_action.
 
+  Instance PolicyParams : PolicyParams := {|
+    ReplacementPolicy.Ifc.name := (StdLibKami.Cam.Ifc.name ++ ".replacementPolicy")%string;
+    ReplacementPolicy.Ifc.num  := StdLibKami.Cam.Ifc.num
+  |}.
+
   Class SimpleCamParams := {
-    regName : string;
-    size : nat;
-    policy: ReplacementPolicy size;
+    (* regName : string; *)
+    (* size : nat; *)
+    policy: @ReplacementPolicy PolicyParams;
     camParamsInst : CamParams
   }.
 
   Section instance.
     Variable (params: SimpleCamParams).
 
-    Local Definition Index : Kind := Bit (Nat.log2_up size).
+    Local Definition Index : Kind := Bit (Nat.log2_up (StdLibKami.Cam.Ifc.num)).
 
     Instance SimpleCam : Cam camParamsInst
       := {| 
            read
              := fun ty tag ctxt
                   => Read xs
-                       :  Array size (Maybe (Pair keyK dataK))
+                       :  Array (StdLibKami.Cam.Ifc.num) (Maybe (Pair keyK dataK))
                        <- regName;
                      utila_acts_find_pkt
                        (map
@@ -40,13 +47,13 @@ Section cam.
                                   "data"
                                     ::= #x @% "data" @% "snd"
                                 } : Maybe dataK @# ty))
-                          (seq 0 size));
+                          (seq 0 (StdLibKami.Cam.Ifc.num)));
 
            write
              := fun ty tag val
                   => LETA index : Index <- @getVictim _ policy ty;
                      Read xs
-                       :  Array size (Maybe (Pair keyK dataK))
+                       :  Array (StdLibKami.Cam.Ifc.num) (Maybe (Pair keyK dataK))
                        <- regName;
                      LET value
                        :  Pair keyK dataK
@@ -61,9 +68,9 @@ Section cam.
            flush
              := fun ty
                   => Write regName
-                       :  Array size (Maybe (Pair keyK dataK))
+                       :  Array (StdLibKami.Cam.Ifc.num) (Maybe (Pair keyK dataK))
                        <- $$(getDefaultConst
-                              (Array size
+                              (Array (StdLibKami.Cam.Ifc.num)
                                 (Maybe
                                 (Pair (@keyK camParamsInst)
                                    (@dataK camParamsInst)))));
@@ -72,7 +79,7 @@ Section cam.
            clear
              := fun ty tag ctxt
                   => Read xs
-                       :  Array size (Maybe (Pair keyK (@dataK camParamsInst)))
+                       :  Array (StdLibKami.Cam.Ifc.num) (Maybe (Pair keyK (@dataK camParamsInst)))
                        <- regName;
                      GatherActions
                        (map
@@ -82,12 +89,12 @@ Section cam.
                                If matchClear tag ctxt (#x @% "data" @% "fst") (#x @% "data" @% "snd")
                                  then
                                    Write regName
-                                     :  Array size (Maybe (Pair keyK dataK))
+                                     :  Array (StdLibKami.Cam.Ifc.num) (Maybe (Pair keyK dataK))
                                      <- #xs@[($i : Index @# ty)
                                           <- unpack (Maybe (Pair keyK dataK)) $0];
                                    Retv;
                                Retv)
-                          (seq 0 size))
+                          (seq 0 (StdLibKami.Cam.Ifc.num)))
                        as _;
                      Retv
          |}.
